pcuic/theories/PCUICCumulativity.v
@@ -23,8 +23,8 @@ Proof.
       exists v', v''. intuition auto. now eapply red_step.
     + destruct IHX as (v' & v'' & (redv & redv') & leqv).
       exists v', v''. intuition auto. now eapply red_step.
-    + todoeta.
-    + todoeta.
+    (* + todoeta.
+    + todoeta. *)
   - intros [v [v' [[redv redv'] Hleq]]]. apply red_alt in redv. apply red_alt in redv'.
     apply clos_rt_rt1n in redv.
     apply clos_rt_rt1n in redv'.
@@ -95,12 +95,12 @@ Proof.
   - destruct IHX as [H1 H2]. split.
     * econstructor 3; eassumption.
     * econstructor 2; eassumption.
-  - destruct IHX as [H1 H2]. split.
+  (* - destruct IHX as [H1 H2]. split.
     * econstructor 4; eassumption.
     * econstructor 5; eassumption.
   - destruct IHX as [H1 H2]. split.
     * econstructor 5; eassumption.
-    * econstructor 4; eassumption.
+    * econstructor 4; eassumption. *)
 Qed.
 
 Lemma conv_cumul {cf:checker_flags} Σ Γ t u :
@@ -121,7 +121,7 @@ Proof.
   intros H%red_alt%clos_rt_rt1n_iff.
   induction H.
   - reflexivity.
-  - econstructor 2; eauto. 
+  - econstructor 2; eauto.
 Qed.
 
 Hint Resolve red_conv : core.
@@ -193,8 +193,8 @@ Proof.
   - eapply red_conv_conv.
     + eapply red1_red in r. eauto.
     + eauto.
-  - eapply conv_eta_r. all: eassumption.
-  - eapply conv_eta_l. all: eassumption.
+  (* - eapply conv_eta_r. all: eassumption.
+  - eapply conv_eta_l. all: eassumption. *)
 Qed.
 
 Lemma conv_alt_red {cf : checker_flags} {Σ : global_env_ext} {Γ : context} {t u : term} :
@@ -207,8 +207,8 @@ Proof.
       exists x, x0; intuition auto. eapply red_step; eauto.
     * destruct IHX as [? [? [? ?]]].
       exists x, x0; intuition auto. eapply red_step; eauto.
-    * todoeta.
-    * todoeta.
+    (* * todoeta.
+    * todoeta. *)
   - destruct 1 as [? [? [[? ?] ?]]].
     eapply red_conv_conv; eauto.
     eapply red_conv_conv_inv; eauto. now constructor.
@@ -259,12 +259,12 @@ Proof.
     econstructor. assumption.
   - eapply cumul_red_r ; try eassumption.
     econstructor. assumption.
-  - eapply cumul_eta_l. 2: eassumption.
+  (* - eapply cumul_eta_l. 2: eassumption.
     destruct e as [na [A [f [π [? ?]]]]]. subst.
     exists na, A, f, (stack_cat π (App x ε)).
     rewrite 2!zipc_stack_cat. cbn. intuition reflexivity.
   - eapply cumul_eta_r. 1: eassumption.
     destruct e as [na [A [f [π [? ?]]]]]. subst.
     exists na, A, f, (stack_cat π (App x ε)).
-    rewrite 2!zipc_stack_cat. cbn. intuition reflexivity.
+    rewrite 2!zipc_stack_cat. cbn. intuition reflexivity. *)
 Qed.
